disk-betree/Betree.dfy
@@ -5,7 +5,7 @@ include "MapSpec.dfy"
 include "Graph.dfy"
 include "BetreeSpec.dfy"
 
-module Betree {
+abstract module Betree {
   import opened BetreeSpec`Internal
   import BI = BetreeBlockInterface
   import MS = MapSpec
